examples.v
@@ -1,0 +1,176 @@
+Require Import Arith.
+Require Import Nat.
+Require Import Bool.
+Require Import bbv.Word.
+Require Import List.
+Require Import Coq_EVM.optimizations.
+Import Optimizations.
+Require Import Coq_EVM.datatypes.
+Import EVM_Def Concrete Abstract Optimizations.
+Require Import Coq_EVM.interpreter.
+Import Interpreter SFS.
+Require Import Coq_EVM.checker.
+Import Checker.
+Import ListNotations.
+
+
+
+Module Examples.
+
+(* CHECKER *)
+Example checker_ex1:
+let optimized_p := [PUSH 32 (natToWord WLen 5)] in
+let p := [PUSH 32 (natToWord WLen 5)] in
+let stack_size := 10 in
+let opt := apply_pipeline_n_times our_optimization_pipeline 20 in
+equiv_checker optimized_p p stack_size opt = true.
+Proof. auto. Qed.
+
+Example checker_ex2:
+let optimized_p := [PUSH 32 (natToWord WLen 6)] in
+let p := [PUSH 32 (natToWord WLen 5)] in
+let stack_size := 10 in
+let opt := apply_pipeline_n_times our_optimization_pipeline 20 in
+equiv_checker optimized_p p stack_size opt = false.
+Proof. auto. Qed.
+
+Example checker_ex3:
+let optimized_p := [PUSH 32 (natToWord WLen 5)] in
+let p := [PUSH 32 (natToWord WLen 5);
+          PUSH 32 (natToWord WLen 6);
+          POP] in
+let stack_size := 10 in
+let opt := apply_pipeline_n_times our_optimization_pipeline 10 in
+equiv_checker optimized_p p stack_size opt = true.
+Proof. auto. Qed.
+
+Example checker_ex4:
+let optimized_p := [PUSH 32 (natToWord WLen 5)] in
+let p := [PUSH 32 (natToWord WLen 0);
+          PUSH 32 (natToWord WLen 5);
+          Opcode ADD] in
+let stack_size := 0 in
+let opt := apply_pipeline_n_times our_optimization_pipeline 10 in
+equiv_checker optimized_p p stack_size opt = true.
+Proof. auto. Qed.
+
+Example checker_ex5:
+let optimized_p := [PUSH 32 (natToWord WLen 5)] in
+let p := [PUSH 32 (natToWord WLen 5);
+          PUSH 32 (natToWord WLen 0);
+          Opcode ADD;
+          PUSH 32 WOne;
+          Opcode MUL] in
+let stack_size := 0 in
+let opt := apply_pipeline_n_times our_optimization_pipeline 10 in
+equiv_checker optimized_p p stack_size opt = true.
+Proof. auto. Qed.
+
+Example checker_ex6:
+let optimized_p := [PUSH 32 (natToWord WLen 5)] in
+let p := [PUSH 32 WOne;
+          PUSH 32 (natToWord WLen 5);
+          PUSH 32 (natToWord WLen 0);
+          Opcode ADD;
+          Opcode MUL] in
+let stack_size := 0 in
+let opt := apply_pipeline_n_times our_optimization_pipeline 10 in
+equiv_checker optimized_p p stack_size opt = true.
+Proof. auto. Qed.
+
+
+
+
+(* CONCRETE EXECUTION *)
+Definition W0  := natToWord WLen 0.
+Definition W1  := natToWord WLen 1.
+Definition W2  := natToWord WLen 2.
+Definition W3  := natToWord WLen 3.
+Definition W4  := natToWord WLen 4.
+Definition W5  := natToWord WLen 5.
+Definition W6  := natToWord WLen 6.
+Definition W7  := natToWord WLen 7.
+Definition W8  := natToWord WLen 8.
+Definition W9  := natToWord WLen 9.
+Definition W10 := natToWord WLen 10.
+
+
+Compute (
+let es := ExState [] empty_nmap empty_nmap
+in let prog := [PUSH 32 W0;
+                PUSH 32 W5;
+                Opcode ADD]
+in concr_interpreter prog es opmap
+).
+
+
+Compute (
+let es := ExState [] empty_nmap empty_nmap
+in let prog := [PUSH 32 W5;
+                PUSH 32 W0;
+                Opcode ADD;
+                PUSH 32 W1;
+                Opcode MUL]
+in concr_interpreter prog es opmap
+).
+
+
+Compute (
+let es := ExState [W7; W7] empty_nmap empty_nmap
+in let prog := [PUSH 32 W0;
+                Opcode ADD;
+                PUSH 32 W2;
+                Opcode MUL]
+in concr_interpreter prog es opmap
+).
+
+
+Compute (
+let es := ExState [W5; W1; W2] empty_nmap empty_nmap
+in let prog := [Opcode ADD;
+                Opcode MUL]
+in concr_interpreter prog es opmap
+).
+
+
+
+
+(* SYMBOLIC EXECUTION *)
+Compute (
+let prog := [PUSH 32 W0;
+             PUSH 32 W5;
+             Opcode ADD]
+in symbolic_exec prog 0 opmap
+).
+
+
+Compute (
+let prog := [PUSH 32 W5;
+             PUSH 32 W0;
+             Opcode ADD;
+             PUSH 32 W1;
+             Opcode MUL]
+in symbolic_exec prog 0 opmap
+).
+
+
+Compute (
+let prog := [PUSH 32 W0;
+             Opcode ADD;
+             PUSH 32 W2;
+             Opcode MUL]
+in symbolic_exec prog 2 opmap
+).
+
+
+Compute (
+let prog := [Opcode ADD;
+             Opcode MUL]
+in symbolic_exec prog 3 opmap
+).
+
+
+
+
+End Examples.
+Import Examples.
