interpreter.v
@@ -1980,7 +1980,60 @@ Definition is_comm_op (opcode: gen_instr) (ops: opm) : bool :=
   | Some (Op true _ _) => true
   | _ => false
   end.
+  
+ 
+Fixpoint flat_stack_elem (e: asfs_stack_val) (m: asfs_map)
+  {struct m} : option flat_asfs_map_val :=
+match e with
+| Val v => Some (FASFSBasicVal (Val v))
+| InStackVar n => Some (FASFSBasicVal (InStackVar n))
+| FreshVar n => 
+    match m with 
+    | (idx, mv)::rm => 
+         if idx =? n then
+         match mv with
+             | ASFSBasicVal (Val v) => Some (FASFSBasicVal (Val v))
+             | ASFSBasicVal (InStackVar n) => Some (FASFSBasicVal (InStackVar n))
+             | ASFSBasicVal (FreshVar n) => flat_stack_elem (FreshVar n) rm
+             | ASFSOp opcode [arg] => match flat_stack_elem arg rm with
+                 | Some farg => Some (FASFSOp opcode [farg])
+                 | _ => None
+                 end
+             | ASFSOp opcode [arg1; arg2] => 
+                 match (flat_stack_elem arg1 rm,
+                        flat_stack_elem arg1 rm) with
+                 | (Some farg1, Some farg2) => Some (FASFSOp opcode [farg1; farg2])
+                 | _ => None
+                 end
+             | _ => None
+             end
+        else flat_stack_elem e rm
+    | _ => None
+    end
+end.
 
+Fixpoint compare_flat_asfs_map_val (e1 e2: flat_asfs_map_val) (ops: opm): bool :=
+match (e1, e2) with
+| (FASFSBasicVal (Val v1), FASFSBasicVal (Val v2)) => weqb v1 v2
+| (FASFSBasicVal (InStackVar v1), FASFSBasicVal (InStackVar v2)) => v1 =? v2
+| (FASFSOp opcode1 [farg1], FASFSOp opcode2 [farg2]) => 
+      (eq_gen_instr opcode1 opcode2) && (compare_flat_asfs_map_val farg1 farg2 ops)
+| (FASFSOp opcode1 [farg11;farg12], FASFSOp opcode2 [farg21; farg22]) => 
+      (eq_gen_instr opcode1 opcode2) && (compare_flat_asfs_map_val farg11 farg21 ops)
+      && (compare_flat_asfs_map_val farg12 farg22 ops)
+  (* TODO add commutativity check *)
+| _ => false
+end.
+
+
+Definition asfs_eq_stack_elem (e1 e2: asfs_stack_val) (m1 m2: asfs_map) 
+  (ops: opm) : bool :=
+match (flat_stack_elem e1 m1, flat_stack_elem e2 m2) with
+| (Some fe1, Some fe2) => compare_flat_asfs_map_val fe1 fe2 ops
+| _ => false
+end.
+
+(*
 (* Overkill: 22 obligations remaining!!! *)
 Program Fixpoint asfs_eq_stack_elem (e1 e2: asfs_stack_val) (m1 m2: asfs_map) 
   (ops: opm) {measure (List.length m1 + List.length m2)} : bool :=
@@ -2135,7 +2188,7 @@ Qed.
 Next Obligation.
   intuition; try discriminate.
 Qed.
-
+*)
 
 
 
